`MSTORE` opcode equivalence (#11)
* Add updated code

* Add `get-arguments.py` script

* `SstoreSummary.lean`: remove `StopSummary` commented import

* `SstoreSummary`: better abstraction of `stack` in `sstore_bypass_private`

* Add `MstoreSummary.lean`

* `MstoreSummary`: prove `EvmYul` and `EVM` `step_mstore_summary`

* `MstoreSummary.lean`: almost prove `X_sstore_summary`

* `MstoreSummary.lean`: finish proof of `X_mstore_summary`

* Move `UInt256` auxiliary lemmas from `MstoreSummary` to `EvmYulInterface`

* Add `scripts/README.md`

* Add `Equivalence/MstoreEquivalence.lean`

* Update generated code

* `StateMap.lean`: cosmetic refactor of some map functions

* `StateMap.lean`: add `memory` and `activeWords` to state map

* Add `Utils/ListByteArrayUtils.lean`

* `EvmYulInterface.lean`: import `ListByteArrayUtils`

* `EvmYulInterface.lean`: add `USize` results

* `EvmYulInterface.lean`: add `COPIED_FROM_EVMYUL` namespace

* `EvmYulInterface.lean`: `Axioms` `ffi_zeroes` and `toBytesBigEndian`

We add the `ffi_zeroes` axiom indicating the expected behavior of the foregin
function interface function `zeroes`
We also assert that `toBytesBigEndian` coincides with the copied definitions
form EvmYul

* `EvmYulInterface.lean`: add theorems for `ffi.zeroes` and `BE` funcs

* `EvmYulInterface.lean`: remove redundant implicit argument

* `EvmYulInterface`: size of conversions to `ByteArray` and `Array`

* `FuncInterface.lean`: add theorems and axiom on functions rewrites

* `MstoreEquivalence.lean`: add `ListbyteArrayUtils` dependency

* `MstoreEquivalence.lean`: add remaining proofs

* `EvmEquivalence.lean`: add `SLOAD` summary and equivalence

* `EvmEquivalence.lean`: add `MSTORE` summary and equivalence

* Update state mapping for `ADD` opcode

* Update state mapping for `PUSH0` opcode

* Update state mapping for `SSTORE` opcode

* Update state mapping for `SLOAD` opcode

* `MstoreEquivalence.lean`: factor out `mstore_activeWords_eq` theorem

* `MstoreEquivalence`: factor out `mstore_memory_write_eq` theorem

* `MstoreEquivalence`: add `X_mstore_equiv` theorem

* `MstoreEquivalence`: fix typo in `step_mstore_equiv` theorem name

* `KEVM2Lean/Rewrite.lean`: format `Rewrites` constructors

scripts/get-arguments.py
@@ -1,0 +1,19 @@
+import re
+import argparse
+
+def arguments(text : str) -> str:
+    return ' '.join(re.findall(r'\{([a-zA-Z0-9_\ ]+)\ :', text))
+
+if __name__ == "__main__":
+	parser = argparse.ArgumentParser(description="Extract text from curly brackets")
+	parser.add_argument("file_path", help="The path to the file containing the text")
+	args = parser.parse_args()
+
+	try:
+	    with open(args.file_path, "r") as file:
+	        text = file.read()
+	        print(arguments(text))
+	except FileNotFoundError:
+	    print(f"Error: The file '{args.file_path}' does not exist")
+	except Exception as e:
+	    print(f"An error occurred: {e}")
