EvmEquivalence/Interfaces/EvmYulInterface.lean
@@ -1,10 +1,99 @@
 import EvmYul.EVM.Semantics
 import EvmEquivalence.Summaries.StopSummary
 import EvmEquivalence.Utils.IntUtils
+import EvmEquivalence.Utils.ListByteArrayUtils
 
 
 open EvmYul
 open EVM
+
+namespace USize
+
+theorem toNat_ofNat_le (n : ℕ) :
+  toNat (@OfNat.ofNat USize n instOfNat) ≤ n := by
+  cases System.Platform.numBits_eq <;> aesop (add simp [toNat]) (add safe (by omega))
+
+theorem toNat_ofNat_eq (n : ℕ) (n_small : n < UInt32.size) :
+  toNat (@OfNat.ofNat USize n instOfNat) = n := by
+  cases System.Platform.numBits_eq <;>
+  aesop (add simp [toNat, UInt32.size]) (add safe (by omega))
+
+end USize
+
+-- We had to copy from EvmYul some functions declared as `private`
+-- We then axiomatically assert that the copied functions and the `private` ones coincide
+section COPIED_FROM_EVMYUL
+
+-- Copied from EvmYul and changed name from `toBytes'` to `toBytes'_ax`
+def toBytes'_ax : ℕ → List UInt8
+  | 0 => []
+  | n@(.succ n') =>
+    let byte : UInt8 := ⟨Nat.mod n UInt8.size, Nat.mod_lt _ (by linarith)⟩
+    have : n / UInt8.size < n' + 1 := by
+      rename_i h
+      rw [h]
+      apply Nat.div_lt_self <;> simp
+    byte :: toBytes'_ax (n / UInt8.size)
+
+-- Copied from EvmYul
+lemma toBytes'_le {k n : ℕ} (h : n < 2 ^ (8 * k)) : (toBytes'_ax n).length ≤ k := by
+  induction k generalizing n with
+  | zero =>
+    simp at h
+    rw [h]
+    simp [toBytes'_ax]
+  | succ e ih =>
+    match n with
+    | .zero => simp [toBytes'_ax]
+    | .succ n =>
+      unfold toBytes'_ax
+      simp [Nat.succ_le_succ_iff]
+      apply ih (Nat.div_lt_of_lt_mul _)
+      rw [Nat.mul_succ, Nat.pow_add] at h
+      linarith
+
+-- Copied from EvmYul
+lemma toBytes'_UInt256_le {n : ℕ} (h : n < UInt256.size) : (toBytes'_ax n).length ≤ 32 := toBytes'_le h
+
+end COPIED_FROM_EVMYUL
+
+namespace Axioms
+
+/-- This should either be provable at some point or a reasonable assumption -/
+axiom ffi_zeroes (len : USize) :
+  ffi.ByteArray.zeroes len = { data := (List.replicate len.toNat 0).toArray }
+
+/-- Needed to bypass `private` attribute of `toBytes'` -/
+axiom toBytesBigEndian_rw (n : ℕ) :
+  EvmYul.toBytesBigEndian n = (List.reverse ∘ toBytes'_ax) n
+
+end Axioms
+
+theorem ffi_zeroes_size (len : USize) :
+  (ffi.ByteArray.zeroes len).size = len.toNat := by
+  simp [Axioms.ffi_zeroes, ByteArray.size]
+
+theorem toBytesBigEndian_lenght_le (n : ℕ) (n_small : n < UInt256.size) :
+  (EvmYul.toBytesBigEndian n).length ≤ 32 := by
+  rw [Axioms.toBytesBigEndian_rw, Function.comp, List.length_reverse]
+  apply toBytes'_UInt256_le; assumption
+
+theorem BE_zero : BE 0 = .empty := by
+  simp [BE, Axioms.toBytesBigEndian_rw, toBytes'_ax]; rfl
+
+theorem BE_size_le_32 (n : ℕ) (h : n < UInt256.size) : (BE n).size ≤ 32 := by
+  simp [BE, Axioms.toBytesBigEndian_rw, List.size_length_eq]
+  apply toBytes'_UInt256_le; assumption
+
+theorem zeroes_size_eq_sub {n : ℕ} (n_small : n < UInt256.size) :
+  ((2 ^ System.Platform.numBits - (BE n).size % 2 ^ System.Platform.numBits + 32) % 2 ^ System.Platform.numBits) = 32 - (BE n).size := by
+  have := BE_size_le_32 n n_small; rw [@Nat.mod_eq_of_lt (BE n).size] <;>
+  cases (System.Platform.numBits_eq) <;> simp_all <;> omega
+
+theorem zeroes_size_eq_32 {n : ℕ} (n_small : n < UInt256.size) :
+  ((2 ^ System.Platform.numBits - (BE n).size % 2 ^ System.Platform.numBits + 32) % 2 ^ System.Platform.numBits) + (BE n).size = 32 := by
+  have := BE_size_le_32 n n_small; rw [@Nat.mod_eq_of_lt (BE n).size] <;>
+  cases (System.Platform.numBits_eq) <;> simp_all <;> omega
 
 namespace UInt256
 
@@ -28,8 +117,16 @@ theorem ofNat_toNat (n_le_size : n < UInt256.size) :
   (UInt256.ofNat n).toNat = n := by
   aesop (add simp [UInt256.ofNat, UInt256.toNat, Id.run, dbgTrace, Fin.ofNat])
 
-theorem ofNat_toSigned {n : ℕ} {p : ℤ} (h : ↑n = p) :
+theorem ofNat_toSigned (h : ↑n = p) :
   UInt256.ofNat n = .toSigned p := by aesop
+
+-- Size of conversions to `ByteArray` and `Array`
+theorem toByteArray_size (val : UInt256) : val.toByteArray.size = 32 := by
+  simp [UInt256.toByteArray, ByteArray.size_append, ffi_zeroes_size]
+  rw [zeroes_size_eq_32]; exact val.val.isLt
+
+theorem toArray_size (n : UInt256) : n.toByteArray.data.size = 32 := by
+  have := UInt256.toByteArray_size; simp_all [ByteArray.size]
 
 -- Arithmetic
 
@@ -51,6 +148,13 @@ theorem zero_add: .ofNat 0 + .ofNat n = UInt256.ofNat n := by
 
 theorem add_succ_mod_size (pos : 0 ≤ p) (size_ok : p + 1 < UInt256.size) : (p + 1) % UInt256.size = p + 1 := by
         rw [Int.mod_cast, Int.toNat_ofNat, Nat.mod_eq_of_lt] <;> aesop (add safe (by omega))
+
+theorem sub_to_fin (n m : UInt256) : n - m = { val := (n.val - m.val)} := rfl
+
+theorem toNat_sub_dist (n m : UInt256) (le_ok : m ≤ n): (n - m).toNat = n.toNat - m.toNat := by
+  rw [sub_to_fin]; simp [UInt256.toNat]; rw [←Fin.sub_val_of_le]; aesop
+
+theorem ofNat_le (n m : UInt256) : (n ≤ m) = (n.toNat ≤ m.toNat) := by aesop
 
 end
 
