EvmEquivalence/Summaries/MstoreSummary.lean
@@ -1,0 +1,232 @@
+import EvmYul.EVM.Semantics
+import EvmYul.EVM.GasConstants
+import EvmEquivalence.Interfaces.EvmYulInterface
+
+open EvmYul
+open EVM
+open EvmYul.State
+
+namespace MstoreSummary
+
+section
+
+variable (gas gasCost : ℕ)
+variable (symStack : Stack UInt256)
+variable (symPc symGasAvailable symRefund offset value : UInt256)
+variable (symActiveWords : UInt256)
+variable (symExecLength : ℕ)
+variable (symReturnData symCode symMemory : ByteArray)
+variable (symAccessedStorageKeys : Batteries.RBSet (AccountAddress × UInt256) Substate.storageKeysCmp)
+variable (symAccounts : AccountMap)
+variable (symCodeOwner : AccountAddress)
+variable (symPerm : Bool)
+
+variable (symValidJumps : Array UInt256)
+
+@[simp]
+abbrev mstoreEVM := @Operation.MSTORE .EVM
+
+@[simp]
+abbrev mstore_instr : Option (Operation .EVM × Option (UInt256 × Nat)) :=
+  some ⟨mstoreEVM, none⟩
+
+@[simp]
+abbrev EVM.step_mstore : Transformer :=
+  EVM.step gas gasCost mstore_instr
+
+@[simp]
+abbrev EvmYul.step_mstore : Transformer :=
+  EvmYul.step mstoreEVM
+
+/--
+Theorem needed to bypass the `private` attribute of `EVM.dispatchBinaryMachineStateOp`
+ -/
+theorem mstore_bypass_private (symState : EVM.State):
+  let ss := {symState with
+  stack := symStack,
+  pc := symPc
+  gasAvailable := symGasAvailable,
+  executionEnv := {symState.executionEnv with
+                  code := symCode,
+                  codeOwner := symCodeOwner
+                  perm := symPerm},
+  accountMap := symAccounts,
+  activeWords := symActiveWords,
+  memory := symMemory,
+  substate := {symState.substate with
+               accessedStorageKeys :=  symAccessedStorageKeys
+               refundBalance := symRefund}
+  returnData := symReturnData,
+  execLength := symExecLength}
+  EvmYul.step_mstore ss =
+  EVM.binaryMachineStateOp EvmYul.MachineState.mstore ss := rfl
+
+/--
+The new amount of `activeWords` based after running `MSTORE` with `offset`
+and `currentAC` amount of active words
+-/
+def mstore_activeWords :=
+  UInt256.ofNat (symActiveWords.toNat ⊔ (offset.toNat + 32 + 31) / 32)
+
+/--
+Writing `value` to `symMemory` starting at `offset`
+-/
+def mstore_memory_write :=
+value.toByteArray.write 0 symMemory offset.toNat 32
+
+theorem EvmYul.step_mstore_summary (symState : EVM.State):
+  let ss := {symState with
+    stack := offset :: value :: symStack,
+    pc := symPc
+    gasAvailable := symGasAvailable,
+    executionEnv := {symState.executionEnv with
+                  code := symCode,
+                  codeOwner := symCodeOwner
+                  perm := symPerm},
+    accountMap := symAccounts,
+    activeWords := symActiveWords,
+    memory := symMemory,
+    substate := {symState.substate with
+                 accessedStorageKeys :=  symAccessedStorageKeys
+                 refundBalance := symRefund}
+    returnData := symReturnData,
+    execLength := symExecLength}
+  EvmYul.step_mstore ss =
+  .ok {ss with
+    stack := symStack,
+    pc := symPc + .ofNat 1
+    memory := mstore_memory_write offset value symMemory,
+    activeWords := mstore_activeWords offset symActiveWords} := by
+  aesop (add simp [mstore_bypass_private])
+
+theorem EVM.step_mstore_summary (gas_pos : 0 < gas) (symState : EVM.State):
+  let ss := {symState with
+    stack := offset :: value :: symStack,
+    pc := symPc
+    gasAvailable := symGasAvailable,
+    executionEnv := {symState.executionEnv with
+                  code := symCode,
+                  codeOwner := symCodeOwner
+                  perm := symPerm},
+    accountMap := symAccounts,
+    activeWords := symActiveWords,
+    memory := symMemory,
+    substate := {symState.substate with
+                 accessedStorageKeys :=  symAccessedStorageKeys
+                 refundBalance := symRefund}
+    returnData := symReturnData,
+    execLength := symExecLength}
+  EVM.step_mstore gas gasCost ss =
+    .ok {ss with
+          stack := symStack,
+          pc := symPc + (.ofNat 1),
+          gasAvailable := symGasAvailable - UInt256.ofNat gasCost,
+          memory := mstore_memory_write offset value symMemory,
+          activeWords := mstore_activeWords offset symActiveWords
+          execLength := symExecLength + 1} := by
+  cases gas; contradiction
+  simp [step_mstore, EVM.step]
+  have srw := EvmYul.step_mstore_summary symStack symPc (symGasAvailable - UInt256.ofNat gasCost) symRefund offset value symActiveWords (symExecLength + 1) symReturnData symCode symMemory
+  simp [EvmYul.step_mstore, Operation.MSTORE] at srw; aesop
+
+@[simp]
+theorem decode_singleton_mstore :
+  decode ⟨#[0x52]⟩ (.ofNat 0) = some ⟨mstoreEVM, none⟩ := rfl
+
+@[simp]
+def value_and_activeWords_gas :=
+  UInt256.ofNat (MachineState.M symActiveWords.toNat value.toNat 32)
+
+@[simp]
+theorem memoryExpansionCost_mstore (symState : EVM.State)
+  (stack_ok : symState.stack = value :: symStack)
+  (symWords_ok : symState.activeWords = symActiveWords):
+  memoryExpansionCost symState mstoreEVM =
+  Cₘ (value_and_activeWords_gas value symActiveWords) - Cₘ symActiveWords := by
+  simp [memoryExpansionCost, memoryExpansionCost.μᵢ']
+  simp [Cₘ, stack_ok, symWords_ok]
+
+/- This theorem is incorrect, needs more constraints to have a positive
+ memory expansion gas cost -/
+/-
+Memory expansion cost for the `MSTORE` opcode is strictly positive
+-/
+/- theorem mec_mstore (symState : EVM.State)
+  (stack_ok : symState.stack = value :: symStack)
+  (words_ok : symState.activeWords = symActiveWords)
+  (aw_gt_0 : 0 < symActiveWords.toNat)
+  (value_big : symActiveWords.toNat < (value.toNat + 32 + 31) / 32)
+  (enough_gas : symActiveWords.toNat ⊔ (value.toNat + 32 + 31) / 32 < UInt256.size):
+  0 < memoryExpansionCost symState mstoreEVM := by
+  simp [memoryExpansionCost, Cₘ, memoryExpansionCost.μᵢ', GasConstants.Gmemory, Cₘ.QuadraticCeofficient, MachineState.M]
+  rw [UInt256.ofNat_toNat] <;> simp [words_ok, stack_ok] <;> try omega
+  apply Nat.add_lt_add
+  . aesop (add safe (by linarith))
+  . simp [max_eq_right (Nat.le_of_lt value_big)] -/
+
+theorem X_mstore_summary (symState : EVM.State)
+                         (symStack_ok : symStack.length < 1024):
+  let ss := {symState with
+    stack := offset :: value :: symStack,
+    pc := .ofNat 0
+    gasAvailable := symGasAvailable,
+    executionEnv := {symState.executionEnv with
+                  code := ⟨#[(0x52 : UInt8)]⟩,
+                  codeOwner := symCodeOwner
+                  perm := symPerm},
+    accountMap := symAccounts,
+    activeWords := symActiveWords,
+    memory := symMemory,
+    substate := {symState.substate with
+                 accessedStorageKeys :=  symAccessedStorageKeys
+                 refundBalance := symRefund}
+    returnData := symReturnData,
+    execLength := symExecLength}
+  -- Assume we have enough gas
+  GasConstants.Gverylow < symGasAvailable.toNat - (memoryExpansionCost ss Operation.MSTORE) →
+  memoryExpansionCost ss Operation.MSTORE < UInt256.size →
+  X symGasAvailable.toNat symValidJumps ss =
+  .ok (.success {ss with
+          stack := symStack,
+          pc := .ofNat 1,
+          gasAvailable := symGasAvailable - .ofNat (memoryExpansionCost ss mstoreEVM) - .ofNat GasConstants.Gverylow
+          memory := mstore_memory_write offset value symMemory,
+          activeWords := mstore_activeWords offset symActiveWords
+          returnData := .empty,
+          execLength := symExecLength + 2} .empty) := by
+  intro ss enoughGas mec_small
+  have gavail_pos : 1 < symGasAvailable.toNat := by
+    rw [GasConstants.Gverylow] at enoughGas; omega
+  cases g_case : symGasAvailable.toNat; omega
+  case succ g_pos =>
+  simp [X, C', δ]
+  have lt_fls_rw {n m : ℕ} (_ : n < m) : (m < n) = False := by
+    simp; apply Nat.ge_of_not_lt; simp; omega
+  simp [(lt_fls_rw enoughGas), α/- , (lt_fls_rw symStack_ok) -/]
+  have fls1 : (symGasAvailable.toNat < memoryExpansionCost ss (@Operation.MSTORE .EVM)) = False :=  by
+    rw [Nat.lt_sub_iff_add_lt] at enoughGas
+    aesop (add safe (by linarith))
+  have decode_rw : ((decode ss.executionEnv.code ss.pc).getD ⟨@Operation.STOP .EVM, none⟩).1 = Operation.MSTORE := rfl
+  have gavail_rw1 : ss.gasAvailable.toNat = symGasAvailable.toNat := rfl
+  have gavail_rw2 : ss.gasAvailable = symGasAvailable := rfl
+  simp [decode_rw, gavail_rw1, gavail_rw2, fls1]
+  simp [InstructionGasGroups.Wcopy, InstructionGasGroups.Wextaccount,
+  InstructionGasGroups.Wzero, InstructionGasGroups.Wbase, InstructionGasGroups.Wverylow]
+  have fls2 : ((symGasAvailable - UInt256.ofNat (memoryExpansionCost ss Operation.MSTORE)).toNat < GasConstants.Gverylow) = False := by
+    apply eq_false_intro; rw [Nat.not_lt]
+    rw [UInt256.toNat_sub_dist, UInt256.ofNat_toNat] <;>
+    aesop (add simp [UInt256.ofNat_le, UInt256.ofNat_toNat])
+  have ss_lt2_f  (n : ℕ) : (n + 1 + 1 < 2) = False := by simp
+  simp [fls2, ss, ss_lt2_f, Nat.not_lt_of_lt symStack_ok]
+  split; contradiction
+  next state n state_ok =>
+  cases state_ok
+  have g_pos_pos : 0 < g_pos := by omega
+  have step_rw (g : UInt256) := (EVM.step_mstore_summary g_pos GasConstants.Gverylow symStack (.ofNat 0) (symGasAvailable - g) symRefund offset value symActiveWords symExecLength symReturnData ⟨#[(0x52 : UInt8)]⟩ symMemory symAccessedStorageKeys symAccounts symCodeOwner symPerm g_pos_pos symState)
+  simp [EVM.step_mstore, mstore_instr, mstoreEVM, ss] at step_rw
+  simp [step_rw, Except.instMonad, Except.bind]
+  rw [X_bad_pc] <;> aesop (add simp [GasConstants.Gverylow]) (add safe (by omega))
+
+end
+
+end MstoreSummary
