EvmEquivalence/Summaries/Push0Summary.lean
@@ -12,9 +12,9 @@ section
 
 variable (gas gasCost : ℕ)
 variable (symStack : Stack UInt256)
-variable (symPc symGasAvailable symRefund : UInt256)
+variable (symPc symGasAvailable symRefund symActiveWords : UInt256)
 variable (symExecLength : ℕ)
-variable (symReturnData symCode : ByteArray)
+variable (symReturnData symCode symMemory : ByteArray)
 variable (symAccessedStorageKeys : Batteries.RBSet (AccountAddress × UInt256) Substate.storageKeysCmp)
 variable (symAccessedStorageKeys : Batteries.RBSet (AccountAddress × UInt256) Substate.storageKeysCmp)
 variable (symAccounts : AccountMap)
@@ -62,7 +62,9 @@ theorem EVM.step_push0_summary (gpos : 0 < gas) (symState : EVM.State):
                   code := symCode,
                   codeOwner := symCodeOwner,
                   perm := symPerm},
-      accountMap := symAccounts
+      accountMap := symAccounts,
+      activeWords := symActiveWords,
+      memory := symMemory,
       substate := {symState.substate with
             accessedStorageKeys :=  symAccessedStorageKeys
             refundBalance := symRefund
@@ -78,6 +80,8 @@ theorem EVM.step_push0_summary (gpos : 0 < gas) (symState : EVM.State):
                   codeOwner := symCodeOwner,
                   perm := symPerm},
     accountMap := symAccounts,
+    activeWords := symActiveWords,
+    memory := symMemory,
     substate := {symState.substate with
             accessedStorageKeys :=  symAccessedStorageKeys
             refundBalance := symRefund
@@ -112,6 +116,8 @@ theorem X_push0_summary (enoughGas : GasConstants.Gbase < symGasAvailable.toNat)
                   codeOwner := symCodeOwner,
                   perm := symPerm},
     accountMap := symAccounts,
+    activeWords := symActiveWords,
+      memory := symMemory,
     substate := {symState.substate with
             accessedStorageKeys :=  symAccessedStorageKeys
             refundBalance := symRefund
@@ -127,6 +133,8 @@ theorem X_push0_summary (enoughGas : GasConstants.Gbase < symGasAvailable.toNat)
                   codeOwner := symCodeOwner,
                   perm := symPerm},
         accountMap := symAccounts,
+        activeWords := symActiveWords,
+        memory := symMemory,
         substate := {symState.substate with
             accessedStorageKeys :=  symAccessedStorageKeys
             refundBalance := symRefund
@@ -144,7 +152,7 @@ theorem X_push0_summary (enoughGas : GasConstants.Gbase < symGasAvailable.toNat)
   rename_i evm _ stateOk; revert stateOk
   simp [pure, Except.pure]; intro evm_eq cost; subst cost evm_eq
   dsimp [Except.instMonad, Except.bind]
-  have step_rw := (@EVM.step_push0_summary g_pos GasConstants.Gbase symStack (.ofNat 0) symGasAvailable symRefund symExecLength symReturnData ⟨#[(0x5F : UInt8)]⟩ symAccessedStorageKeys symAccounts symCodeOwner symPerm gPos)
+  have step_rw := (@EVM.step_push0_summary g_pos GasConstants.Gbase symStack (.ofNat 0) symGasAvailable symRefund symActiveWords symExecLength symReturnData ⟨#[(0x5F : UInt8)]⟩ symMemory symAccessedStorageKeys symAccounts symCodeOwner symPerm gPos)
   rw [EVM.step_push0, push0_instr] at step_rw; simp [step_rw]
   rw [X_bad_pc] <;> aesop (add simp [GasConstants.Gbase]) (add safe (by omega))
 
